Isabelle/04_Composed_operations/Until_support.thy
@@ -1,0 +1,403 @@
+theory Until_support
+  imports 
+"../T_03_Basic_programs"
+"Arbitrary_repetition"
+begin
+section \<open>Until support for top\<close>
+
+subsection \<open>Step cases\<close>
+lemma until_decomp_1: "until_support a C b 0 n \<equiv>\<^sub>p until_support a C b 0 0 \<union>\<^sub>p until_support a C b (Suc 0) n"
+  apply (simp add: until_support_def)                   
+proof (induction n)
+  case 0
+  have right_1: "loop (b \<sslash>\<^sub>p (- C)) (Suc 0) 0 \<setminus>\<^sub>p C \<equiv>\<^sub>p Fail (S b)"
+    by (metis corestriction_prop equiv_is_transitive fail_compose_l loop_l2_01 restriction_state)
+  from right_1 have right_2: "a; loop (b \<sslash>\<^sub>p (- C)) (Suc 0) 0 \<setminus>\<^sub>p C \<equiv>\<^sub>p Fail (S b)"
+    by (metis equiv_def composition_def corestriction_state fail_compose_r loop_l2_01 restriction_state)
+  from right_2 have right_3: "a ; Skip (S b) \<setminus>\<^sub>p C \<union>\<^sub>p a ; loop (b \<sslash>\<^sub>p (- C)) (Suc 0) 0 \<setminus>\<^sub>p C \<equiv>\<^sub>p a ; Skip (S b) \<setminus>\<^sub>p C \<union>\<^sub>p Fail (S b)"
+    by (simp add: equiv_is_reflexive equivalence_is_maintained_by_choice)
+  from right_3 have right_4: "a ; Skip (S b) \<setminus>\<^sub>p C \<union>\<^sub>p a ; loop (b \<sslash>\<^sub>p (- C)) (Suc 0) 0 \<setminus>\<^sub>p C \<equiv>\<^sub>p a ; Skip (S b) \<setminus>\<^sub>p C"
+    by (meson equiv_is_transitive fail_union_r)
+  from right_2 have left_1: "a ; loop (b \<sslash>\<^sub>p (- C)) 0 0 \<setminus>\<^sub>p C \<equiv>\<^sub>p a ; Skip (Pre (b \<sslash>\<^sub>p (- C))) \<setminus>\<^sub>p C"
+    by (simp add: equals_equiv_relation_3 restrict_p_def)
+  have l1: "a ; Fail (S b) \<setminus>\<^sub>p C \<equiv>\<^sub>p Fail (S b)"
+    using right_2 by auto
+  from right_3 show ?case
+    by (auto simp: equiv_def Skip_def Fail_def composition_def corestrict_p_def corestrict_r_def choice_def restr_post_def restrict_r_def)
+next
+  case (Suc n)
+  assume IH: "a ; loop (b \<sslash>\<^sub>p (- C)) 0 n \<setminus>\<^sub>p C \<equiv>\<^sub>p a ; Skip (Pre (b \<sslash>\<^sub>p (- C))) \<setminus>\<^sub>p C \<union>\<^sub>p a ; loop (b \<sslash>\<^sub>p (- C)) (Suc 0) n \<setminus>\<^sub>p C"
+  have l2: "a ; loop (b \<sslash>\<^sub>p (- C)) 0 (Suc n) \<setminus>\<^sub>p C \<equiv>\<^sub>p a ; (Skip (Pre (b \<sslash>\<^sub>p (- C))) \<union>\<^sub>p loop (b \<sslash>\<^sub>p (- C)) (Suc 0) (Suc n)) \<setminus>\<^sub>p C"
+    by (metis One_nat_def equals_equiv_relation_3 equivalence_is_maintained_by_composition equivalence_is_maintained_by_corestriction loop_l6 zero_less_Suc)
+  have l3: "a ; (Skip (Pre (b \<sslash>\<^sub>p (- C))) \<union>\<^sub>p loop (b \<sslash>\<^sub>p (- C)) (Suc 0) (Suc n)) \<setminus>\<^sub>p C \<equiv>\<^sub>p ((a ; Skip (Pre (b \<sslash>\<^sub>p (- C)))) \<union>\<^sub>p (a ; loop (b \<sslash>\<^sub>p (- C)) (Suc 0) (Suc n))) \<setminus>\<^sub>p C"
+    using corestrict_compose equiv_is_symetric equivalence_is_maintained_by_corestriction equiv_is_transitive compose_distrib1_3 by blast
+  then have l4: "((a ; Skip (Pre (b \<sslash>\<^sub>p (- C)))) \<union>\<^sub>p (a ; loop (b \<sslash>\<^sub>p (- C)) (Suc 0) (Suc n))) \<setminus>\<^sub>p C \<equiv>\<^sub>p ((a ; Skip (Pre (b \<sslash>\<^sub>p (- C))) \<setminus>\<^sub>p C) \<union>\<^sub>p (a ; loop (b \<sslash>\<^sub>p (- C)) (Suc 0) (Suc n) \<setminus>\<^sub>p C))"
+    by (meson corestrict_union corestrict_compose equiv_is_transitive equivalence_is_maintained_by_choice)
+  from compose_distrib1_3 corestrict_union l2 show ?case
+    using equiv_is_transitive l3 l4 by blast
+qed
+
+lemma until_decomp_2: "until_support a C b 0 (Suc n) \<equiv>\<^sub>p until_support a C b 0 n \<union>\<^sub>p until_support a C b (Suc n) (Suc n)"
+proof (induction n)
+  case 0
+  then show ?case
+    using until_decomp_1 by auto
+next
+  case (Suc n)
+  assume IH: "until_support a C b 0 (Suc n) \<equiv>\<^sub>p until_support a C b 0 n \<union>\<^sub>p until_support a C b (Suc n) (Suc n)"
+  have t2: "until_support a C b 0 (Suc (Suc n)) \<equiv>\<^sub>p (a ; (loop (b\<sslash>\<^sub>p(-C)) 0 (Suc n))\<setminus>\<^sub>p C) \<union>\<^sub>p (a ; (loop (b\<sslash>\<^sub>p(-C)) (Suc (Suc n)) (Suc (Suc n)))\<setminus>\<^sub>p C)"
+    apply (auto simp: until_support_def)
+  proof -
+    have l1: "a ; ((b \<sslash>\<^sub>p (- C)) \<^bold>^ n ; (b \<sslash>\<^sub>p (- C) ; b \<sslash>\<^sub>p (- C))) \<setminus>\<^sub>p C \<equiv>\<^sub>p a ; (Fail (S b) \<union>\<^sub>p (b \<sslash>\<^sub>p (- C)) \<^bold>^ n ; (b \<sslash>\<^sub>p (- C) ; b \<sslash>\<^sub>p (- C))) \<setminus>\<^sub>p C"
+      by (simp add: equiv_is_reflexive equiv_is_symetric equivalence_is_maintained_by_composition equivalence_is_maintained_by_corestriction fail_union_l)
+    have l2: "a ; (loop (b \<sslash>\<^sub>p (- C)) 0 n \<union>\<^sub>p b \<sslash>\<^sub>p (- C) ; (b \<sslash>\<^sub>p (- C)) \<^bold>^ n) \<setminus>\<^sub>p C \<equiv>\<^sub>p a ; (loop (b \<sslash>\<^sub>p (- C)) 0 n \<union>\<^sub>p b \<sslash>\<^sub>p (- C) ; (b \<sslash>\<^sub>p (- C)) \<^bold>^ n) \<setminus>\<^sub>p C"
+      by (simp add: equiv_is_reflexive)
+    from l1 l2 until_simplification_1 show "a ; ((b \<sslash>\<^sub>p (- C)) \<^bold>^ n ; (b \<sslash>\<^sub>p (- C) ; b \<sslash>\<^sub>p (- C)) \<union>\<^sub>p (loop (b \<sslash>\<^sub>p (- C)) 0 n \<union>\<^sub>p (b \<sslash>\<^sub>p (- C)) \<^bold>^ n ; b \<sslash>\<^sub>p (- C))) \<setminus>\<^sub>p C \<equiv>\<^sub>p
+    a ; (loop (b \<sslash>\<^sub>p (- C)) 0 n \<union>\<^sub>p (b \<sslash>\<^sub>p (- C)) \<^bold>^ n ; b \<sslash>\<^sub>p (- C)) \<setminus>\<^sub>p C \<union>\<^sub>p a ; (Fail (S b) \<union>\<^sub>p (b \<sslash>\<^sub>p (- C)) \<^bold>^ n ; (b \<sslash>\<^sub>p (- C) ; b \<sslash>\<^sub>p (- C))) \<setminus>\<^sub>p C"
+      by (smt (verit, ccfv_threshold) choice_commute equiv_is_symetric equiv_is_transitive equivalence_is_maintained_by_choice)
+  qed
+  then show "until_support a C b 0 (Suc (Suc n)) \<equiv>\<^sub>p until_support a C b 0 (Suc n) \<union>\<^sub>p until_support a C b (Suc (Suc n)) (Suc (Suc n))"
+    by (simp add: until_support_def)
+qed
+
+lemma until_decomp_3: "s \<le> f \<Longrightarrow> until_support a C b s f \<equiv>\<^sub>p until_support a C b s s \<union>\<^sub>p until_support a C b (Suc s) f"
+  apply (simp add: until_support_def)
+proof (induction s)
+  case 0
+  from until_decomp_1 show ?case
+    by (metis until_support_def)
+next
+  case (Suc s)
+  assume IH: "s \<le> f \<Longrightarrow>  a ; loop (b \<sslash>\<^sub>p (- C)) s f \<setminus>\<^sub>p C \<equiv>\<^sub>p a ; loop (b \<sslash>\<^sub>p (- C)) s s \<setminus>\<^sub>p C \<union>\<^sub>p a ; loop (b \<sslash>\<^sub>p (- C)) (Suc s) f \<setminus>\<^sub>p C"
+  assume a1: "Suc s \<le> f"
+  have IH2: "a ; loop (b \<sslash>\<^sub>p (- C)) s f \<setminus>\<^sub>p C \<equiv>\<^sub>p a ; loop (b \<sslash>\<^sub>p (- C)) s s \<setminus>\<^sub>p C \<union>\<^sub>p a ; loop (b \<sslash>\<^sub>p (- C)) (Suc s) f \<setminus>\<^sub>p C"
+    by (simp add: IH Suc_leD a1)
+  from IH2 have l1: "a ; loop (b \<sslash>\<^sub>p (- C)) (Suc s) f \<setminus>\<^sub>p C \<equiv>\<^sub>p a ; (loop (b \<sslash>\<^sub>p (- C)) (Suc s) (Suc s) \<union>\<^sub>p loop (b \<sslash>\<^sub>p (- C)) (Suc (Suc s)) f) \<setminus>\<^sub>p C"
+    by (metis a1 equiv_is_reflexive equivalence_is_maintained_by_composition equivalence_is_maintained_by_corestriction le_refl loop_l5)
+  then have l2: "a ; (loop (b \<sslash>\<^sub>p (- C)) (Suc s) (Suc s) \<union>\<^sub>p loop (b \<sslash>\<^sub>p (- C)) (Suc (Suc s)) f) \<setminus>\<^sub>p C \<equiv>\<^sub>p a ; loop (b \<sslash>\<^sub>p (- C)) (Suc s) (Suc s) \<setminus>\<^sub>p C \<union>\<^sub>p a ; loop (b \<sslash>\<^sub>p (- C)) (Suc (Suc s)) f \<setminus>\<^sub>p C"
+    using compose_distrib1_3 corestrict_union equiv_is_reflexive equiv_is_transitive equivalence_is_maintained_by_composition by blast
+  then show ?case
+    using equiv_is_transitive l1 by blast
+qed
+
+lemma until_decomp_4: "s \<le> f \<Longrightarrow> until_support a C b s (Suc f) \<equiv>\<^sub>p until_support a C b (Suc f) (Suc f) \<union>\<^sub>p until_support a C b s f"
+proof (induction f)
+  case 0
+  assume a1: "s \<le> 0"
+  have l1: "s = 0"
+    using a1 by auto
+  from loop_l5 l1 show ?case
+    by (simp add: until_decomp_2)
+next
+  case (Suc f)
+  assume IH: "s \<le> f \<Longrightarrow> until_support a C b s (Suc f) \<equiv>\<^sub>p until_support a C b (Suc f) (Suc f) \<union>\<^sub>p until_support a C b s f"
+  assume a1: "s \<le> Suc f"
+  from loop_l3 have l1: "(a ; (loop (b\<sslash>\<^sub>p(-C)) s (Suc (Suc f)))\<setminus>\<^sub>p C) \<equiv>\<^sub>p a ; (((b\<sslash>\<^sub>p(-C))\<^bold>^(Suc (Suc f))) \<union>\<^sub>p (loop (b\<sslash>\<^sub>p(-C)) s (Suc f)))\<setminus>\<^sub>p C"
+    using a1 equiv_is_reflexive by auto
+  have l2: "until_support a C b s (Suc (Suc f)) \<equiv>\<^sub>p a ; (((b\<sslash>\<^sub>p(-C))\<^bold>^(Suc (Suc f))) \<union>\<^sub>p (loop (b\<sslash>\<^sub>p(-C)) s (Suc f)))\<setminus>\<^sub>p C"
+    by (metis l1 until_support_def)
+  have l3: "until_support a C b (Suc (Suc f)) (Suc (Suc f)) \<union>\<^sub>p until_support a C b s (Suc f) \<equiv>\<^sub>p a ; ((b\<sslash>\<^sub>p(-C))\<^bold>^(Suc (Suc f)) \<union>\<^sub>p loop (b\<sslash>\<^sub>p(-C)) s (Suc f))\<setminus>\<^sub>p C"
+  proof -
+    have l3_1: "until_support a C b (Suc (Suc f)) (Suc (Suc f)) \<equiv>\<^sub>p a ; ((b\<sslash>\<^sub>p(-C))\<^bold>^(Suc (Suc f))) \<setminus>\<^sub>p C"
+      by (metis equiv_is_reflexive equivalence_is_maintained_by_composition equivalence_is_maintained_by_corestriction loop_l2_1 until_support_def)
+    have l3_2: "until_support a C b s (Suc f) \<equiv>\<^sub>p a ; (loop (b\<sslash>\<^sub>p(-C)) s (Suc f))\<setminus>\<^sub>p C"
+      by (simp add: equiv_is_reflexive until_support_def)
+    from l3_1 l3_2 have l3_3: "until_support a C b (Suc (Suc f)) (Suc (Suc f)) \<union>\<^sub>p until_support a C b s (Suc f) \<equiv>\<^sub>p a ; ((b\<sslash>\<^sub>p(-C))\<^bold>^(Suc (Suc f))) \<setminus>\<^sub>p C \<union>\<^sub>p a ; (loop (b\<sslash>\<^sub>p(-C)) s (Suc f))\<setminus>\<^sub>p C"
+      using equivalence_is_maintained_by_choice by blast
+    then show ?thesis
+      by (meson compose_distrib1_3 corestrict_union equiv_is_reflexive equiv_is_symetric equiv_is_transitive equivalence_is_maintained_by_composition)
+  qed
+  then show "until_support a C b s (Suc (Suc f)) \<equiv>\<^sub>p until_support a C b (Suc (Suc f)) (Suc (Suc f)) \<union>\<^sub>p until_support a C b s (Suc f)"
+    using equiv_is_symetric equiv_is_transitive l2 by blast
+qed
+
+subsection \<open>Decomposition\<close>
+
+lemma until_decomp_5: "0 \<le> k \<Longrightarrow> k \<le> n \<Longrightarrow> until_support a C b 0 n \<equiv>\<^sub>p until_support a C b 0 k \<union>\<^sub>p until_support a C b (Suc k) n"
+proof (induction k)
+  case 0
+  then show ?case
+    by (simp add: until_decomp_1)
+next
+  case (Suc k)
+  assume IH: "0 \<le> k \<Longrightarrow> k \<le> n \<Longrightarrow> until_support a C b 0 n \<equiv>\<^sub>p until_support a C b 0 k \<union>\<^sub>p until_support a C b (Suc k) n"
+  assume a1: "0 \<le> Suc k"
+  assume a2: "Suc k \<le> n"
+  have l1: "until_support a C b 0 (Suc k) \<equiv>\<^sub>p until_support a C b 0 k \<union>\<^sub>p until_support a C b (Suc k) (Suc k)"
+    by (simp add: until_decomp_2)
+  have l2: "until_support a C b 0 n \<equiv>\<^sub>p until_support a C b 0 k \<union>\<^sub>p until_support a C b (Suc k) n"
+    using IH a2 by auto
+  have l3: "until_support a C b (Suc k) n \<equiv>\<^sub>p until_support a C b (Suc k) (Suc k) \<union>\<^sub>p until_support a C b (Suc (Suc k)) n"
+    by (simp add: a2 until_decomp_3)
+  then have l4: "until_support a C b 0 n \<equiv>\<^sub>p until_support a C b 0 k \<union>\<^sub>p (until_support a C b (Suc k) (Suc k) \<union>\<^sub>p until_support a C b (Suc (Suc k)) n)"
+    by (meson equiv_is_symetric equiv_is_transitive equivalence_is_maintained_by_choice l2 until_decomp_1)
+  from IH a1 a2 show "until_support a C b 0 n \<equiv>\<^sub>p until_support a C b 0 (Suc k) \<union>\<^sub>p until_support a C b (Suc (Suc k)) n"
+    by (smt (verit, ccfv_SIG) choice_assoc_1 equiv_is_reflexive equiv_is_symetric equiv_is_transitive equivalence_is_maintained_by_choice l1 l4)
+qed
+
+lemma until_decomp_6: "s \<le> k \<Longrightarrow> k \<le> f \<Longrightarrow> until_support a C b s f \<equiv>\<^sub>p until_support a C b s k \<union>\<^sub>p until_support a C b (Suc k) f"
+proof (induction k)
+  case 0
+  then show ?case
+    by (simp add: until_decomp_1)
+next
+  case (Suc k)
+  assume IH: "s \<le> k \<Longrightarrow> k \<le> f \<Longrightarrow> until_support a C b s f \<equiv>\<^sub>p until_support a C b s k \<union>\<^sub>p until_support a C b (Suc k) f"
+  assume a1: "s \<le> Suc k"
+  assume a2: "Suc k \<le> f"
+  from a2 have l1: "k \<le> f" by auto
+  then show "until_support a C b s f \<equiv>\<^sub>p until_support a C b s (Suc k) \<union>\<^sub>p until_support a C b (Suc (Suc k)) f"
+  proof (cases "s \<le> k")
+    case True
+    have l2: "until_support a C b s f \<equiv>\<^sub>p until_support a C b s k \<union>\<^sub>p until_support a C b (Suc k) f"
+      by (simp add: IH True l1)
+    have l3: "until_support a C b (Suc k) f \<equiv>\<^sub>p until_support a C b (Suc k) (Suc k) \<union>\<^sub>p until_support a C b (Suc (Suc k)) f"
+      by (simp add: a2 until_decomp_3)
+    have l4: "until_support a C b s (Suc k) \<equiv>\<^sub>p until_support a C b s k \<union>\<^sub>p until_support a C b (Suc k) (Suc k)"
+      using True until_decomp_4 by fastforce
+    have l5: "until_support a C b s f \<equiv>\<^sub>p until_support a C b s k \<union>\<^sub>p (until_support a C b (Suc k) (Suc k) \<union>\<^sub>p until_support a C b (Suc (Suc k)) f)"
+      using equiv_is_reflexive equiv_is_transitive equivalence_is_maintained_by_choice l2 l3 by blast
+    have l6: "until_support a C b s f \<equiv>\<^sub>p (until_support a C b s k \<union>\<^sub>p until_support a C b (Suc k) (Suc k)) \<union>\<^sub>p until_support a C b (Suc (Suc k)) f"
+      by (metis choice_assoc_1 l5)
+    from l2 l3 l4 l5 l6 show "until_support a C b s f \<equiv>\<^sub>p until_support a C b s (Suc k) \<union>\<^sub>p until_support a C b (Suc (Suc k)) f"
+      by (meson equiv_is_reflexive equiv_is_symetric equiv_is_transitive equivalence_is_maintained_by_choice)
+  next
+    case False
+    then show ?thesis
+      by (metis a1 a2 le_SucE until_decomp_3)
+  qed
+qed
+
+lemma until_decomp_7: "s = f \<Longrightarrow> until_support a C b s f \<equiv>\<^sub>p a ; ((b \<sslash>\<^sub>p (- C))\<^bold>^f) \<setminus>\<^sub>p C"
+  by (simp add: equiv_is_reflexive equivalence_is_maintained_by_composition equivalence_is_maintained_by_corestriction loop_l2_1 until_support_def)
+
+lemma until_support_feasible: "all_feasible [a, b] \<Longrightarrow> is_feasible (until_support a C b s f)"
+proof (induction f)
+  case 0
+  then show ?case
+    by (simp add: until_support_def compose_feasible corestrict_feasible fail_is_feasible skip_is_feasible)
+next
+  case (Suc f)
+  assume IH: "all_feasible [a, b] \<Longrightarrow> is_feasible (until_support a C b s f)"
+  assume a1: "all_feasible [a, b]"
+  from a1 IH have l1: "is_feasible (until_support a C b s f)" by simp
+  then show ?case
+  proof (cases "s \<le> f")
+    case True
+    assume a2: "s \<le> f"
+    from a2 until_decomp_4 until_decomp_7 have l2: "until_support a C b s (Suc f) \<equiv>\<^sub>p until_support a C b s f \<union>\<^sub>p until_support a C b (Suc f) (Suc f)"
+      using choice_commute by fastforce
+    from l2 until_decomp_7 have l3: "until_support a C b s (Suc f) \<equiv>\<^sub>p until_support a C b s f \<union>\<^sub>p (a ; ((b \<sslash>\<^sub>p (- C))\<^bold>^(Suc f)) \<setminus>\<^sub>p C)"
+      by (smt (verit, ccfv_SIG) equals_equiv_relation_3 equiv_is_transitive equivalence_is_maintained_by_choice)
+    have l4: "is_feasible (a ; ((b \<sslash>\<^sub>p (- C))\<^bold>^(Suc f)) \<setminus>\<^sub>p C)"
+      by (meson a1 all_feasible.simps(2) compose_feasible corestrict_feasible fixed_rep_feasibility restrict_feasible)
+    then show ?thesis
+      by (meson all_feasible.simps(1) all_feasible.simps(2) union_feasible equiv_is_symetric equiv_maintains_feasiblity l1 l3)
+  next
+    case False
+    assume a2: "\<not> s \<le> f"
+    from a2 have l1: "s>f" by simp
+    then show ?thesis
+    proof (cases "s = Suc f")
+      case True
+      assume a3: "s = Suc f"
+      from a3 have l2: "until_support a C b s (Suc f) \<equiv>\<^sub>p until_support a C b s s"
+        by (simp add: equiv_is_reflexive)
+      have l3: "is_feasible (until_support a C b s s)"
+        apply (simp add: until_support_def)
+        by (meson a1 all_feasible.simps(2) arbitrary_rep_feasibility compose_feasible corestrict_feasible restrict_feasible verit_comp_simplify1(2))
+      from a3 l2 l3 show ?thesis by simp
+    next
+      case False
+      assume a3: "f < s"
+      assume a4: " s \<noteq> Suc f"
+      from a3 a4 have "s > Suc f" by simp
+      then show ?thesis
+        apply (simp add: until_support_def)
+        by (meson a1 all_feasible.simps(2) compose_feasible corestrict_feasible fail_is_feasible)
+    qed
+  qed
+qed
+
+theorem equiv_is_maintained_by_until_support_1: 
+  assumes "a\<^sub>1 \<equiv>\<^sub>p a\<^sub>2"
+      and "b\<^sub>1 \<equiv>\<^sub>p b\<^sub>2"
+      and "S b\<^sub>1 = S b\<^sub>2"
+      and "all_feasible [b\<^sub>1, b\<^sub>2]"
+    shows "until_support a\<^sub>1 C b\<^sub>1 s f \<equiv>\<^sub>p until_support a\<^sub>2 C b\<^sub>2 s f"
+  apply (auto simp: until_support_def)
+  apply (induction f)
+  apply (auto) [1]
+  apply (simp add: assms(1) assms(3) equals_equiv_relation_3 equivalence_is_maintained_by_composition)
+  apply (metis (no_types, opaque_lifting) Definitions.equiv_def assms(1) assms(2) equivalence_is_maintained_by_composition equivalence_is_maintained_by_restriction)
+proof -
+  fix f assume IH: "a\<^sub>1 ; loop (b\<^sub>1 \<sslash>\<^sub>p (- C)) s f \<setminus>\<^sub>p C \<equiv>\<^sub>p a\<^sub>2 ; loop (b\<^sub>2 \<sslash>\<^sub>p (- C)) s f \<setminus>\<^sub>p C"
+  have l1: "b\<^sub>1 \<sslash>\<^sub>p (- C) \<equiv>\<^sub>p b\<^sub>2 \<sslash>\<^sub>p (- C)"
+    by (simp add: assms(2) equivalence_is_maintained_by_restriction)
+  have l2: "S (b\<^sub>1 \<sslash>\<^sub>p (- C)) = S (b\<^sub>2 \<sslash>\<^sub>p (- C))"
+    by (simp add: assms(3))
+  from l1 l2 assms (2) assms (3) assms (4)  have l3: "loop (b\<^sub>1 \<sslash>\<^sub>p (- C)) s (Suc f) \<equiv>\<^sub>p loop (b\<^sub>2 \<sslash>\<^sub>p (- C)) s (Suc f)"
+    by (meson all_feasible.simps(2) equiv_is_maintained_by_arbitrary_repetition_1 restrict_feasible)
+  show "a\<^sub>1 ; loop (b\<^sub>1 \<sslash>\<^sub>p (- C)) s (Suc f) \<setminus>\<^sub>p C \<equiv>\<^sub>p a\<^sub>2 ; loop (b\<^sub>2 \<sslash>\<^sub>p (- C)) s (Suc f) \<setminus>\<^sub>p C"
+    using assms(1) equivalence_is_maintained_by_composition equivalence_is_maintained_by_corestriction l3 by blast
+qed
+
+theorem equiv_is_maintained_by_until_support_2: 
+  assumes "a\<^sub>1 \<equiv>\<^sub>p a\<^sub>2"
+      and "b\<^sub>1 \<equiv>\<^sub>p b\<^sub>2"
+      and "0<s"
+      and "all_feasible [b\<^sub>1, b\<^sub>2]"
+    shows "until_support a\<^sub>1 C b\<^sub>1 s f \<equiv>\<^sub>p until_support a\<^sub>2 C b\<^sub>2 s f"
+  apply (auto simp: until_support_def)
+  apply (induction f)
+  apply (auto) [1]
+  apply (simp add: assms(1) assms(3) equals_equiv_relation_3 equivalence_is_maintained_by_composition)
+  apply (simp add: assms(1) equivalence_is_maintained_by_composition equivalence_is_maintained_by_corestriction fail_is_equivalent_independant_of_arg)
+  using assms(3) apply auto[1]
+proof -
+  fix f assume IH: "a\<^sub>1 ; loop (b\<^sub>1 \<sslash>\<^sub>p (- C)) s f \<setminus>\<^sub>p C \<equiv>\<^sub>p a\<^sub>2 ; loop (b\<^sub>2 \<sslash>\<^sub>p (- C)) s f \<setminus>\<^sub>p C"
+  have l1: "b\<^sub>1 \<sslash>\<^sub>p (- C) \<equiv>\<^sub>p b\<^sub>2 \<sslash>\<^sub>p (- C)"
+    by (simp add: assms(2) equivalence_is_maintained_by_restriction)
+  from l1 assms (2) assms (3) assms (4)  have l3: "loop (b\<^sub>1 \<sslash>\<^sub>p (- C)) s (Suc f) \<equiv>\<^sub>p loop (b\<^sub>2 \<sslash>\<^sub>p (- C)) s (Suc f)"
+    by (metis all_feasible.simps(2) assms(3) assms(4) equiv_is_maintained_by_arbitrary_repetition_2 l1 restrict_feasible)
+  show "a\<^sub>1 ; loop (b\<^sub>1 \<sslash>\<^sub>p (- C)) s (Suc f) \<setminus>\<^sub>p C \<equiv>\<^sub>p a\<^sub>2 ; loop (b\<^sub>2 \<sslash>\<^sub>p (- C)) s (Suc f) \<setminus>\<^sub>p C"
+    using assms(1) equivalence_is_maintained_by_composition equivalence_is_maintained_by_corestriction l3 by blast
+qed
+
+theorem bad_index_is_fail_support: "f < s \<Longrightarrow> until_support a C b s f \<equiv>\<^sub>p Fail {}"
+proof -
+  assume a1: "f < s"
+  then have "loop (b\<sslash>\<^sub>p(-C)) s f \<equiv>\<^sub>p Fail {}"
+    by (simp add: bad_index_is_fail_arbitrary)
+  then have l1: "until_support a C b s f \<equiv>\<^sub>p a ; (Fail {})\<setminus>\<^sub>p C"
+    by (simp add: equiv_is_reflexive equivalence_is_maintained_by_composition equivalence_is_maintained_by_corestriction until_support_def)
+  have l2: "a ; (Fail {})\<setminus>\<^sub>p C \<equiv>\<^sub>p Fail {}"
+    by (metis corestrict_idem fail_compose_r infeas_corestriction)
+  then show "until_support a C b s f \<equiv>\<^sub>p Fail {}"
+    using equiv_is_transitive l1 by blast
+qed
+
+theorem bad_index_range_support: "f < s \<Longrightarrow> Range_p (until_support a C b s f) = {}"
+proof -
+  assume a1: "f < s"
+  then have "until_support a C b s f \<equiv>\<^sub>p Fail {}"
+    by (simp add: bad_index_is_fail_support)
+  then show "Range_p (until_support a C b s f) = {}"
+    by (metis range_of_fail same_range_p_3)
+qed
+
+theorem until_support_decomp:
+  assumes "s\<le>s'" and "f'\<le>f "
+  shows "until_support a C b s f \<equiv>\<^sub>p until_support a C b s f \<union>\<^sub>p until_support a C b s' f'"
+proof (cases "s'\<le>f'")
+  case True
+  then show ?thesis using assms
+  proof (induction f)
+    case 0
+    then show ?case by (auto simp: until_support_def composition_def equiv_def restr_post_def Fail_def restrict_r_def corestrict_p_def restrict_p_def corestrict_r_def)
+  next
+    case (Suc f)
+    assume IH: "s' \<le> f' \<Longrightarrow> s \<le> s' \<Longrightarrow> f' \<le> f \<Longrightarrow> until_support a C b s f \<equiv>\<^sub>p until_support a C b s f \<union>\<^sub>p until_support a C b s' f'"
+    assume a1: "s \<le> s'"
+    assume a2: "f' \<le> Suc f"
+    assume a4: "s' \<le> f'"
+    have a3: "s \<le> Suc f"
+      using a1 a2 a4 by auto
+    obtain suc where o1: "suc = until_support a C b s (Suc f)" by simp
+    obtain here where o2: "here = until_support a C b s f" by simp
+    obtain head where o3: "head = until_support a C b s (s'-1)" by simp
+    obtain prime where o4: "prime = until_support a C b s' f'" by simp
+    obtain tail where o5: "tail = until_support a C b (Suc f') (Suc f)" by simp
+    obtain ptail where o6: "ptail = until_support a C b s' (Suc f)" by simp
+    show "until_support a C b s (Suc f) \<equiv>\<^sub>p until_support a C b s (Suc f) \<union>\<^sub>p until_support a C b s' f'"
+    proof (cases "s=0")
+      case True
+      assume "s=0"
+      have l2: "suc \<equiv>\<^sub>p head \<union>\<^sub>p ptail"
+      proof (cases "s'=s")
+        case True
+        then have "s'-1 = 0"
+          by (simp add: \<open>s = 0\<close>)
+        then have "head \<equiv>\<^sub>p until_support a C b 0 0"
+          by (simp add: \<open>s = 0\<close> equals_equiv_relation_3 o3)
+        have "ptail = until_support a C b 0 (Suc f)"
+          by (simp add: True \<open>s = 0\<close> o6)
+        obtain butfst where o8: "butfst = until_support a C b (Suc 0) (Suc f)" by simp
+        have "suc \<equiv>\<^sub>p head \<union>\<^sub>p butfst" using \<open>s = 0\<close> until_decomp_3
+          by (metis \<open>s' - 1 = 0\<close> a3 o1 o3 o8)
+        then have "suc \<equiv>\<^sub>p (head \<union>\<^sub>p head) \<union>\<^sub>p butfst" using choice_idem_3
+          by (smt (verit, del_insts) Definitions.equiv_def equivalence_is_maintained_by_choice)
+        then have "suc \<equiv>\<^sub>p head \<union>\<^sub>p (head \<union>\<^sub>p butfst)"
+          by (metis choice_assoc_1)
+        then show ?thesis
+          by (metis True \<open>head \<equiv>\<^sub>p until_support a C b 0 0\<close> \<open>suc \<equiv>\<^sub>p head \<union>\<^sub>p butfst\<close> equiv_is_symetric equiv_is_transitive equivalence_is_maintained_by_choice o1 o6)
+      next
+        case False
+        obtain temp where o7: "temp = (s'-1)" by simp
+        have "s'>0"
+          using False a1 by auto
+        have l1: "head = until_support a C b s temp"
+          by (simp add: o3 o7)
+        have l2: "ptail = until_support a C b (Suc temp) (Suc f)"
+          by (simp add: \<open>0 < s'\<close> o6 o7)
+        then show ?thesis
+          by (metis (full_types) False Suc_diff_1 \<open>0 < s'\<close> a1 a2 a4 diff_le_self l1 le_SucE le_trans o1 o7 until_decomp_6)
+      qed
+      have l3: "ptail \<equiv>\<^sub>p prime \<union>\<^sub>p tail"
+        by (simp add: a2 a4 o4 o5 o6 until_decomp_6) 
+      have l4: "suc \<equiv>\<^sub>p (head \<union>\<^sub>p prime) \<union>\<^sub>p tail"
+        by (metis choice_assoc_1 equiv_is_reflexive equiv_is_transitive equivalence_is_maintained_by_choice l2 l3)
+      have l5: "suc \<equiv>\<^sub>p ((head \<union>\<^sub>p (prime \<union>\<^sub>p prime)) \<union>\<^sub>p tail)"
+        by (meson choice_idem_3 equiv_is_symetric equiv_is_transitive equivalence_is_maintained_by_choice l4)
+      have l6: "suc \<equiv>\<^sub>p ((head \<union>\<^sub>p prime) \<union>\<^sub>p tail) \<union>\<^sub>p prime"
+        by (metis choice_assoc_1 choice_commute l5)
+      have l7: "suc \<equiv>\<^sub>p suc \<union>\<^sub>p prime"
+        by (smt (verit) choice_assoc_1 choice_commute choice_idem_3 equiv_is_symetric equiv_is_transitive equivalence_is_maintained_by_choice l4 l5)
+      then show ?thesis
+        by (simp add: o1 o4)
+    next
+      case False
+      have l2: "suc \<equiv>\<^sub>p head \<union>\<^sub>p ptail"
+      proof (cases "s'=s")
+        case True
+        then have "head \<equiv>\<^sub>p Fail{}" using o3 False
+          by (simp add: bad_index_is_fail_support)
+        then show ?thesis using True o6 o1
+          by (meson equiv_is_symetric equiv_is_transitive equivalence_is_maintained_by_choice fail_union_l)
+      next
+        case False
+        obtain temp where o7: "temp = (s'-1)" by simp
+        have "s'>0"
+          using False a1 by auto
+        have l1: "head = until_support a C b s temp"
+          by (simp add: o3 o7)
+        have l2: "ptail = until_support a C b (Suc temp) (Suc f)"
+          by (simp add: \<open>0 < s'\<close> o6 o7)
+        then show ?thesis
+          by (metis (full_types) False Suc_diff_1 \<open>0 < s'\<close> a1 a2 a4 diff_le_self l1 le_SucE le_trans o1 o7 until_decomp_6)
+      qed
+      have l3: "ptail \<equiv>\<^sub>p prime \<union>\<^sub>p tail"
+        by (simp add: a2 a4 o4 o5 o6 until_decomp_6) 
+      have l4: "suc \<equiv>\<^sub>p (head \<union>\<^sub>p prime) \<union>\<^sub>p tail"
+        by (metis choice_assoc_1 equiv_is_reflexive equiv_is_transitive equivalence_is_maintained_by_choice l2 l3)
+      have l5: "suc \<equiv>\<^sub>p ((head \<union>\<^sub>p (prime \<union>\<^sub>p prime)) \<union>\<^sub>p tail)"
+        by (meson choice_idem_3 equiv_is_symetric equiv_is_transitive equivalence_is_maintained_by_choice l4)
+      have l6: "suc \<equiv>\<^sub>p ((head \<union>\<^sub>p prime) \<union>\<^sub>p tail) \<union>\<^sub>p prime"
+        by (metis choice_assoc_1 choice_commute l5)
+      have l7: "suc \<equiv>\<^sub>p suc \<union>\<^sub>p prime"
+        by (smt (verit) choice_assoc_1 choice_commute choice_idem_3 equiv_is_symetric equiv_is_transitive equivalence_is_maintained_by_choice l4 l5)
+      then show ?thesis
+        by (simp add: o1 o4)
+    qed
+  qed
+next
+  case False
+  have "f' < s'"
+    using False by auto
+  moreover have "until_support a C b s' f' \<equiv>\<^sub>p Fail {}"
+    by (simp add: bad_index_is_fail_support calculation)
+  then show ?thesis
+    by (meson equiv_is_symetric equiv_is_transitive equivalence_is_maintained_by_choice fail_union_r)
+qed
+
+end
