Isabelle/05_Properties/Loop_invariant.thy
@@ -31,42 +31,42 @@ lemma loop_correct_1: "is_loop_invariant I a C b \<Longrightarrow> Range_p (a ; 
       using l1 same_range_p_3 by auto
   qed
 
-lemma loop_correct_2: "is_loop_invariant I a C b \<Longrightarrow> Range_p (while_support a C b n n) \<subseteq> I"
+lemma loop_correct_2: "is_loop_invariant I a C b \<Longrightarrow> Range_p (until_support a C b n n) \<subseteq> I"
   proof (induction n)
     case 0
-    then show ?case by (auto simp: while_support_def composition_def Skip_def restrict_p_def restrict_r_def corestrict_p_def corestrict_r_def Range_p_def)
+    then show ?case by (auto simp: until_support_def composition_def Skip_def restrict_p_def restrict_r_def corestrict_p_def corestrict_r_def Range_p_def)
   next
     case (Suc n)
-    assume IH: "is_loop_invariant I a C b \<Longrightarrow> Range_p (while_support a C b n n) \<subseteq> I"
+    assume IH: "is_loop_invariant I a C b \<Longrightarrow> Range_p (until_support a C b n n) \<subseteq> I"
     assume a2: "is_loop_invariant I a C b"
-    from IH a2 have IH2: "Range_p (while_support a C b n n) \<subseteq> I" by simp
+    from IH a2 have IH2: "Range_p (until_support a C b n n) \<subseteq> I" by simp
     then have IH_exp: "\<forall>x y. x \<in> Pre a \<and> (x, y) \<in> post (a; ((b\<sslash>\<^sub>p(-C))\<^bold>^n)) \<longrightarrow> y \<in> I"
       by (meson a2 corestriction_invariant_preserve fixed_repetition_invariant_preserve invariant_preserve is_loop_invariant_def)
     then have IH_exp_2: "\<forall>x y. x \<in> Pre a \<and> (x, y) \<in> post (a; ((b\<sslash>\<^sub>p(-C))\<^bold>^(Suc n))) \<longrightarrow> y \<in> I"
       by (meson a2 fixed_repetition_invariant_preserve invariant_preserve is_loop_invariant_def)
     then have IH_exp_3: "\<forall>x y. x \<in> Pre a \<and> (x, y) \<in> post (a; ((b\<sslash>\<^sub>p(-C))\<^bold>^(Suc n)) \<setminus>\<^sub>p C) \<longrightarrow> y \<in> I"
       by (meson a2 corestriction_invariant_preserve fixed_repetition_invariant_preserve invariant_preserve is_loop_invariant_def)
-    have l1: "while_support a C b (Suc n) (Suc n) \<equiv>\<^sub>p a; ((b\<sslash>\<^sub>p(-C))\<^bold>^(Suc n)) \<setminus>\<^sub>p C"
-      using while_decomp_7 by blast
-    then have "\<forall>x y. x \<in> Pre a \<and> (x, y) \<in> post (while_support a C b (Suc n) (Suc n)) \<longrightarrow> y \<in> I"
-      by (metis (full_types) IH_exp_3 composition_pre knowing_pre_composition range_p_explicit_1 range_p_explicit_2 same_range_p_3 subsetD while_support_def)
-    then show "Range_p (while_support a C b (Suc n) (Suc n)) \<subseteq> I"
-      by (metis composition_pre in_mono range_p_explicit_1 subsetI while_support_def)
+    have l1: "until_support a C b (Suc n) (Suc n) \<equiv>\<^sub>p a; ((b\<sslash>\<^sub>p(-C))\<^bold>^(Suc n)) \<setminus>\<^sub>p C"
+      using until_decomp_7 by blast
+    then have "\<forall>x y. x \<in> Pre a \<and> (x, y) \<in> post (until_support a C b (Suc n) (Suc n)) \<longrightarrow> y \<in> I"
+      by (metis (full_types) IH_exp_3 composition_pre knowing_pre_composition range_p_explicit_1 range_p_explicit_2 same_range_p_3 subsetD until_support_def)
+    then show "Range_p (until_support a C b (Suc n) (Suc n)) \<subseteq> I"
+      by (metis composition_pre in_mono range_p_explicit_1 subsetI until_support_def)
   qed
 
-lemma loop_correct_3: "s\<le>f \<Longrightarrow> is_loop_invariant I a C b \<Longrightarrow> Range_p (while_support a C b s f) \<subseteq> I"
+lemma loop_correct_3: "s\<le>f \<Longrightarrow> is_loop_invariant I a C b \<Longrightarrow> Range_p (until_support a C b s f) \<subseteq> I"
   apply (induction f)
-   apply (smt (verit) in_mono le_numeral_extra(3) loop_correct_2 range_while_loop_2 subsetI while_conncetion)
+   apply (smt (verit) in_mono le_numeral_extra(3) loop_correct_2 range_until_loop_2 subsetI until_conncetion)
 proof -
-  fix f assume IH: "s \<le> f \<Longrightarrow> is_loop_invariant I a C b \<Longrightarrow> Range_p (while_support a C b s f) \<subseteq> I"
+  fix f assume IH: "s \<le> f \<Longrightarrow> is_loop_invariant I a C b \<Longrightarrow> Range_p (until_support a C b s f) \<subseteq> I"
   assume a1: "is_loop_invariant I a C b"
   assume a2: " s \<le> Suc f"
-  show "Range_p (while_support a C b s (Suc f)) \<subseteq> I"
+  show "Range_p (until_support a C b s (Suc f)) \<subseteq> I"
   proof (cases "s\<le>f")
     case True
-    from IH a1 True have l1: "Range_p (while_support a C b s f) \<subseteq> I" by simp
-    from True have l2: "while_support a C b s (Suc f) \<equiv>\<^sub>p while_support a C b s f \<union>\<^sub>p while_support a C b (Suc f) (Suc f)"
-      by (metis choice_commute while_decomp_4)
+    from IH a1 True have l1: "Range_p (until_support a C b s f) \<subseteq> I" by simp
+    from True have l2: "until_support a C b s (Suc f) \<equiv>\<^sub>p until_support a C b s f \<union>\<^sub>p until_support a C b (Suc f) (Suc f)"
+      by (metis choice_commute until_decomp_4)
     then show ?thesis
       by (smt (verit) l1 a1 choice_range_p_prop_2 loop_correct_2 same_range_p_3 subsetD subsetI)
   next
@@ -77,23 +77,23 @@ proof -
 qed
 
 
-theorem loop_correct: "is_loop_invariant I a C b \<Longrightarrow> Range_p (while_loop a C b n) \<subseteq> C \<inter> I" \<comment> \<open>Loop_correct\<close>
+theorem loop_correct: "is_loop_invariant I a C b \<Longrightarrow> Range_p (until_loop a C b n) \<subseteq> C \<inter> I" \<comment> \<open>Loop_correct\<close>
   apply (auto)
 proof -
   assume a1: "is_loop_invariant I a C b"
-  fix n x assume a2: "x \<in> Range_p (while_loop a C b n)"
+  fix n x assume a2: "x \<in> Range_p (until_loop a C b n)"
   from a1 a2 show "x \<in> C"
-    apply (auto simp: while_loop_def)
+    apply (auto simp: until_loop_def)
     by (meson Corestriction.corestrict_prop_1 in_mono range_decreases_composition)
 next
-  fix x assume a2: "x \<in> Range_p (while_loop a C b n)"
+  fix x assume a2: "x \<in> Range_p (until_loop a C b n)"
   assume a1: "is_loop_invariant I a C b"
   
   from a1 a2 have "x \<in> C"
-    apply (auto simp: while_loop_def)
+    apply (auto simp: until_loop_def)
     by (meson Corestriction.corestrict_prop_1 in_mono range_decreases_composition)
   from a1 a2 show "x \<in> I"
-    by (metis bot_nat_0.extremum in_mono loop_correct_3 while_conncetion)
+    by (metis bot_nat_0.extremum in_mono loop_correct_3 until_conncetion)
 qed
 
 end
